```
Boolean theorems with one variable
    Identity
      Theorem: B • 1 = B
        ✓ 0 • 1 = 0
        ✓ 1 • 1 = 1
      Dual: B + 0 = B
        ✓ 0 + 0 = 0
        ✓ 1 + 0 = 1
    Null element
      Theorem: B • 0 = 0
        ✓ 0 • 0 = 0
        ✓ 1 • 0 = 0
      Dual: B + 1 = 1
        ✓ 0 + 1 = 1
        ✓ 1 + 1 = 1
    Idempotency
      Theorem: B • B = B
        ✓ 0 • 0 = 0
        ✓ 1 • 1 = 1
      Dual: B + B = B
        ✓ 0 + 0 = 0
        ✓ 1 + 1 = 1
    Involution
      Theorem: B = ¯¯B
        ✓ 0 = ¯¯0
        ✓ 1 = ¯¯1
    Complements
      Theorem: B • ¯B = 0
        ✓ 0 • ¯0 = 0
        ✓ 1 • ¯1 = 0
      Dual: B + ¯B = 1
        ✓ 0 + ¯0 = 1
        ✓ 1 + ¯1 = 1
  Boolean theorems of several variables
    Commutativity
      Theorem: B • C = B • C
        ✓ 0 • 0 = 0 • 0
        ✓ 0 • 1 = 0 • 1
        ✓ 1 • 0 = 1 • 0
        ✓ 1 • 1 = 1 • 1
      Dual: B + C = B + C
        ✓ 0 + 0 = 0 + 0
        ✓ 0 + 1 = 0 + 1
        ✓ 1 + 0 = 1 + 0
        ✓ 1 + 1 = 1 + 1
    Associativity
      Theorem: (B • C) • D = B • (C • D)
        ✓ (0 • 0) • 0 = 0 • (0 • 0)
        ✓ (0 • 0) • 1 = 0 • (0 • 1)
        ✓ (0 • 1) • 0 = 0 • (1 • 0)
        ✓ (0 • 1) • 1 = 0 • (1 • 1)
        ✓ (1 • 0) • 0 = 1 • (0 • 0)
        ✓ (1 • 0) • 1 = 1 • (0 • 1)
        ✓ (1 • 1) • 0 = 1 • (1 • 0)
        ✓ (1 • 1) • 1 = 1 • (1 • 1)
      Dual: (B + C) + D = B + (C + D)
        ✓ (0 + 0) + 0 = 0 + (0 + 0)
        ✓ (0 + 0) + 1 = 0 + (0 + 1)
        ✓ (0 + 1) + 0 = 0 + (1 + 0)
        ✓ (0 + 1) + 1 = 0 + (1 + 1)
        ✓ (1 + 0) + 0 = 1 + (0 + 0)
        ✓ (1 + 0) + 1 = 1 + (0 + 1)
        ✓ (1 + 1) + 0 = 1 + (1 + 0)
        ✓ (1 + 1) + 1 = 1 + (1 + 1)
    Distributivity
      Theorem: (B • C) + (B • D) = B • (C + D)
        ✓ (0 • 0) + (0 • 0) = 0 • (0 + 0)
        ✓ (0 • 0) + (0 • 1) = 0 • (0 + 1)
        ✓ (0 • 1) + (0 • 0) = 0 • (1 + 0)
        ✓ (0 • 1) + (0 • 1) = 0 • (1 + 1)
        ✓ (1 • 0) + (1 • 0) = 1 • (0 + 0)
        ✓ (1 • 0) + (1 • 1) = 1 • (0 + 1)
        ✓ (1 • 1) + (1 • 0) = 1 • (1 + 0)
        ✓ (1 • 1) + (1 • 1) = 1 • (1 + 1)
      Dual: (B + C) • (B + D) = B + (C • D)
        ✓ (0 + 0) • (0 + 0) = 0 + (0 • 0)
        ✓ (0 + 0) • (0 + 1) = 0 + (0 • 1)
        ✓ (0 + 1) • (0 + 0) = 0 + (1 • 0)
        ✓ (0 + 1) • (0 + 1) = 0 + (1 • 1)
        ✓ (1 + 0) • (1 + 0) = 1 + (0 • 0)
        ✓ (1 + 0) • (1 + 1) = 1 + (0 • 1)
        ✓ (1 + 1) • (1 + 0) = 1 + (1 • 0)
        ✓ (1 + 1) • (1 + 1) = 1 + (1 • 1)
    Covering
      Theorem: B • (B + C) = B
        ✓ 0 • (0 + 0) = 0
        ✓ 0 • (0 + 1) = 0
        ✓ 1 • (1 + 0) = 1
        ✓ 1 • (1 + 1) = 1
      Dual: B + (B • C) = B
        ✓ 0 + (0 • 0) = 0
        ✓ 0 + (0 • 1) = 0
        ✓ 1 + (1 • 0) = 1
        ✓ 1 + (1 • 1) = 1
    Combining
      Theorem: (B • C) + (B • ¯C) = B
        ✓ (0 • 0) + (0 • ¯0) = 0
        ✓ (0 • 1) + (0 • ¯1) = 0
        ✓ (1 • 0) + (1 • ¯0) = 1
        ✓ (1 • 1) + (1 • ¯1) = 1
      Dual: (B + C) • (B + ¯C) = B
        ✓ (0 + 0) • (0 + ¯0) = 0
        ✓ (0 + 1) • (0 + ¯1) = 0
        ✓ (1 + 0) • (1 + ¯0) = 1
        ✓ (1 + 1) • (1 + ¯1) = 1
    Consensus
      Theorem: (B • C) + (¯B • D) + (C • D) = B • C + ¯B • D
        ✓ (0 • 0) + (¯0 • 0) + (0 • 0) = 0 • 0 + ¯0 • 0
        ✓ (0 • 0) + (¯0 • 1) + (0 • 1) = 0 • 0 + ¯0 • 1
        ✓ (0 • 1) + (¯0 • 0) + (1 • 0) = 0 • 1 + ¯0 • 0
        ✓ (0 • 1) + (¯0 • 1) + (1 • 1) = 0 • 1 + ¯0 • 1
        ✓ (1 • 0) + (¯1 • 0) + (0 • 0) = 1 • 0 + ¯1 • 0
        ✓ (1 • 0) + (¯1 • 1) + (0 • 1) = 1 • 0 + ¯1 • 1
        ✓ (1 • 1) + (¯1 • 0) + (1 • 0) = 1 • 1 + ¯1 • 0
        ✓ (1 • 1) + (¯1 • 1) + (1 • 1) = 1 • 1 + ¯1 • 1
      Dual: (B + C) • (¯B + D) • (C + D) = B + C • ¯B + D
        ✓ (0 + 0) • (¯0 + 0) • (0 + 0) = 0 + 0 • ¯0 + 0
        ✓ (0 + 0) • (¯0 + 1) • (0 + 1) = 0 + 0 • ¯0 + 1
        ✓ (0 + 1) • (¯0 + 0) • (1 + 0) = 0 + 1 • ¯0 + 0
        ✓ (0 + 1) • (¯0 + 1) • (1 + 1) = 0 + 1 • ¯0 + 1
        ✓ (1 + 0) • (¯1 + 0) • (0 + 0) = 1 + 0 • ¯1 + 0
        ✓ (1 + 0) • (¯1 + 1) • (0 + 1) = 1 + 0 • ¯1 + 1
        ✓ (1 + 1) • (¯1 + 0) • (1 + 0) = 1 + 1 • ¯1 + 0
        ✓ (1 + 1) • (¯1 + 1) • (1 + 1) = 1 + 1 • ¯1 + 1
    De Morgan's Theorem
      Theorem: ¯(B • C • D ...) = (¯B + ¯C + ¯D ...)
        ✓ ¯(0 • 0 • 0 ...) = (¯0 + ¯0 + ¯0 ...)
        ✓ ¯(0 • 0 • 1 ...) = (¯0 + ¯0 + ¯1 ...)
        ✓ ¯(0 • 1 • 0 ...) = (¯0 + ¯1 + ¯0 ...)
        ✓ ¯(0 • 1 • 1 ...) = (¯0 + ¯1 + ¯1 ...)
        ✓ ¯(1 • 0 • 0 ...) = (¯1 + ¯0 + ¯0 ...)
        ✓ ¯(1 • 0 • 1 ...) = (¯1 + ¯0 + ¯1 ...)
        ✓ ¯(1 • 1 • 0 ...) = (¯1 + ¯1 + ¯0 ...)
        ✓ ¯(1 • 1 • 1 ...) = (¯1 + ¯1 + ¯1 ...)
      Dual: ¯(B + C + D ...) = (¯B • ¯C • ¯D)
        ✓ ¯(0 + 0 + 0 ...) = (¯0 • ¯0 • ¯0)
        ✓ ¯(0 + 0 + 1 ...) = (¯0 • ¯0 • ¯1)
        ✓ ¯(0 + 1 + 0 ...) = (¯0 • ¯1 • ¯0)
        ✓ ¯(0 + 1 + 1 ...) = (¯0 • ¯1 • ¯1)
        ✓ ¯(1 + 0 + 0 ...) = (¯1 • ¯0 • ¯0)
        ✓ ¯(1 + 0 + 1 ...) = (¯1 • ¯0 • ¯1)
        ✓ ¯(1 + 1 + 0 ...) = (¯1 • ¯1 • ¯0)
        ✓ ¯(1 + 1 + 1 ...) = (¯1 • ¯1 • ¯1)
```
